HeapLang/PrimitiveLaws.thy
@@ -1,0 +1,10 @@
+theory PrimitiveLaws
+imports State
+begin
+
+section \<open> Basic laws for HeapLang programs \<close>
+text \<open> Based on https://gitlab.mpi-sws.org/iris/iris/-/blob/master/iris_heap_lang/primitive_laws.v \<close>
+
+
+
+end
