IrisCore/LogicSyntax.thy
@@ -1,0 +1,104 @@
+theory LogicSyntax
+imports Main
+begin
+(* The Coq formalization also used the empty type but I have no idea why 
+  or whether HOL has such a type. M is the carrier type of the underlying camera. *)
+datatype logic_type = PropT | M |EmptyT | UnitT | SumT logic_type logic_type
+  | ProdT "logic_type\<times>logic_type" | FunT logic_type logic_type
+
+datatype 'x logic_term = 
+  Var string
+| Abort "'x logic_term"
+| Unit
+| Prod "'x logic_term\<times>'x logic_term"
+| Fst "'x logic_term"
+| Snd "'x logic_term"
+| Abs string logic_type "'x logic_term"
+| App "'x logic_term" "'x logic_term"
+| Left "'x logic_term"
+| Right "'x logic_term"
+| Match "'x logic_term" string "'x logic_term" string "'x logic_term"
+| Const 'x
+| Core "'x logic_term"
+| Comp "'x logic_term" "'x logic_term"
+| FalseTrm
+| TrueTrm
+| EqTrm logic_type "'x logic_term" "'x logic_term"
+| Impl "'x logic_term" "'x logic_term"
+| Conj "'x logic_term" "'x logic_term"
+| Disj "'x logic_term" "'x logic_term"
+| Sep "'x logic_term" "'x logic_term"
+| Wand "'x logic_term" "'x logic_term"
+| Guarded string logic_type "'x logic_term"
+| Exists string logic_type "'x logic_term"
+| Forall string logic_type "'x logic_term"
+| Own "'x logic_term"
+| Valid "'x logic_term"
+| Persistent "'x logic_term"
+| Plain "'x logic_term"
+| Later "'x logic_term"
+| Upd "'x logic_term"
+
+(* Variable substitution in logic terms *)
+fun logic_subst :: "(string \<Rightarrow> string) \<Rightarrow> 'x logic_term \<Rightarrow> 'x logic_term" where
+  "logic_subst f (Var x) = Var (f x)"
+| "logic_subst f (Prod (x,y)) = Prod (logic_subst f x, logic_subst f y)"
+| "logic_subst f (Fst t) = Fst (logic_subst f t)"
+| "logic_subst f (Snd t) = Snd (logic_subst f t)"
+| "logic_subst f (Abs x \<tau> t) = Abs x \<tau> (logic_subst (f(x:=x)) t)"
+| "logic_subst f (App t1 t2) = App (logic_subst f t1) (logic_subst f t2)"
+| "logic_subst f (Left t) = Left (logic_subst f t)"
+| "logic_subst f (Right t) = Right (logic_subst f t)"
+| "logic_subst f (Match t x l y r) = 
+  Match (logic_subst f t) x (logic_subst (f(x:=x)) l) y (logic_subst (f(y:=y)) r)"
+| "logic_subst f (Core t) = Core (logic_subst f t)"
+| "logic_subst f (Comp t1 t2) = Comp (logic_subst f t1) (logic_subst f t2)"
+| "logic_subst f (EqTrm \<tau> t1 t2) = EqTrm \<tau> (logic_subst f t1) (logic_subst f t2)"
+| "logic_subst f (Impl t1 t2) = Impl (logic_subst f t1) (logic_subst f t2)"
+| "logic_subst f (Conj t1 t2) = Conj (logic_subst f t1) (logic_subst f t2)"
+| "logic_subst f (Disj t1 t2) = Disj (logic_subst f t1) (logic_subst f t2)"
+| "logic_subst f (Sep t1 t2) = Sep (logic_subst f t1) (logic_subst f t2)"
+| "logic_subst f (Wand t1 t2) = Wand (logic_subst f t1) (logic_subst f t2)"
+| "logic_subst f (Guarded x \<tau> t) = Guarded x \<tau> (logic_subst (f(x:=x)) t)"
+| "logic_subst f (Exists x \<tau> t) = Exists x \<tau> (logic_subst (f(x:=x)) t)"
+| "logic_subst f (Forall x \<tau> t) = Forall x \<tau> (logic_subst (f(x:=x)) t)"
+| "logic_subst f (Own t) = Own (logic_subst f t)"
+| "logic_subst f (Valid t) = Valid (logic_subst f t)"
+| "logic_subst f (Persistent t) = Persistent (logic_subst f t)"
+| "logic_subst f (Plain t) = Plain (logic_subst f t)"
+| "logic_subst f (Later t) = Later (logic_subst f t)"
+| "logic_subst f (Upd t) = Upd (logic_subst f t)"
+| "logic_subst _ t = t"
+
+(* The variable x can only appear under the later modality. *)
+fun guarded :: "string \<Rightarrow> 'x logic_term \<Rightarrow> bool" where
+  "guarded _ (Later (Var _)) = True"
+| "guarded x (Abort t) = guarded x t"
+| "guarded x (Prod (t1,t2)) = (guarded x t1 \<and> guarded x t2)"
+| "guarded x (Fst t) = guarded x t"
+| "guarded x (Snd t) = guarded x t"
+| "guarded x (Abs y _ t) = ((x=y) \<or> guarded x t)"
+| "guarded x (Left t) = guarded x t"
+| "guarded x (Right t) = guarded x t"
+| "guarded x (Match t y l z r) = (guarded x t \<and> ((x=y) \<or> guarded x l) \<and> ((x=z) \<or> guarded x r))"
+| "guarded x (Core t) = guarded x t"
+| "guarded x (Comp t1 t2) = (guarded x t1 \<and> guarded x t2)"
+| "guarded x (EqTrm _ t1 t2) = (guarded x t1 \<and> guarded x t2)"
+| "guarded x (Impl t1 t2) = (guarded x t1 \<and> guarded x t2)"
+| "guarded x (Conj t1 t2) = (guarded x t1 \<and> guarded x t2)"
+| "guarded x (Disj t1 t2) = (guarded x t1 \<and> guarded x t2)"
+| "guarded x (Sep t1 t2) = (guarded x t1 \<and> guarded x t2)"
+| "guarded x (Wand t1 t2) = (guarded x t1 \<and> guarded x t2)"
+| "guarded x (Guarded y _ t) = ((x=y) \<or> guarded x t)"
+| "guarded x (Exists y _ t) = ((x=y) \<or> guarded x t)"
+| "guarded x (Forall y _ t) = ((x=y) \<or> guarded x t)"
+| "guarded x (Own t) = guarded x t"
+| "guarded x (Valid t) = guarded x t"
+| "guarded x (Persistent t) = guarded x t"
+| "guarded x (Plain t) = guarded x t"
+| "guarded x (Later t) = guarded x t"
+| "guarded x (Upd t) = guarded x t"
+| "guarded _ (Var _) = False"
+| "guarded _ _ = True"
+
+end
